verified/ARMunroll.i.dfy
@@ -1,0 +1,194 @@
+// REQUIRES: TEST
+// RUN: %DAFNY /compile:0 %s %DARGS
+include "ARMspartan.dfy"
+
+abstract module UnrollableCode {
+
+import opened ARMspartan_unrollablecode = ARMspartan
+
+//////////////////////////////////////////////////
+// THINGS TO BE FILLED IN BY CONCRETE MODULE
+//////////////////////////////////////////////////
+
+type GenericConstantState
+type GenericCodeParameters
+type GenericAuxiliaryState
+
+function method GenericIterationCount() : int
+    ensures GenericIterationCount() >= 0;
+
+predicate GenericFramingInvariant(sp_s0:sp_state, sp_sM:sp_state)
+    requires ValidState(sp_s0);
+    requires ValidState(sp_sM);
+    ensures sp_s0 == sp_sM ==> GenericFramingInvariant(sp_s0, sp_sM);
+
+lemma lemma_GenericFramingInvariantTransitivity(sp_s1:sp_state, sp_s2:sp_state, sp_s3:sp_state)
+    requires ValidState(sp_s1);
+    requires ValidState(sp_s2);
+    requires ValidState(sp_s3);
+    requires GenericFramingInvariant(sp_s1, sp_s2);
+    requires GenericFramingInvariant(sp_s2, sp_s3);
+    ensures  GenericFramingInvariant(sp_s1, sp_s3);
+
+predicate GenericStateInvariant(c:GenericConstantState, s:sp_state, aux:GenericAuxiliaryState, i:int, p:GenericCodeParameters)
+
+function method GenericCodeIteration(i:int, p:GenericCodeParameters) : code
+    requires 0 <= i < GenericIterationCount();
+
+lemma sp_lemma_GenericIterationPreservesInvariants(
+    sp_b0:sp_codes,
+    sp_s0:sp_state,
+    sp_sN:sp_state,
+    i:int,
+    p:GenericCodeParameters
+    ) returns (
+    sp_bM:sp_codes,
+    sp_sM:sp_state
+    )
+    requires 0 <= i < GenericIterationCount();
+    requires sp_require(sp_b0, GenericCodeIteration(i, p), sp_s0, sp_sN);
+    ensures  sp_ensure(sp_b0, sp_bM, sp_s0, sp_sM, sp_sN);
+    ensures  forall sp_id:sp_int, c:GenericConstantState, aux0:GenericAuxiliaryState {:trigger sp_trigger_GenericUnrolledChunk(sp_id, c, aux0)} ::
+                 sp_trigger_GenericUnrolledChunk(sp_id, c, aux0) ==> sp_spec_GenericUnrolledChunk(c, aux0, sp_s0, sp_sM, i, i+1, p);
+    ensures  GenericFramingInvariant(sp_s0, sp_sM);
+
+//////////////////////////////////////////////////
+// DERIVED THINGS
+//////////////////////////////////////////////////
+
+function sp_trigger_GenericUnrolledChunk(
+    sp_id:sp_int,
+    c:GenericConstantState,
+    aux:GenericAuxiliaryState
+    ):sp_bool
+{
+    true
+}
+
+function {:opaque} sp_spec_GenericUnrolledChunk(
+    c:GenericConstantState,
+    aux0:GenericAuxiliaryState,
+    sp_s0:sp_state,
+    sp_sM:sp_state,
+    i0:int,
+    iM:int,
+    p:GenericCodeParameters
+    ):sp_bool
+{
+    sp_s0.ok && GenericStateInvariant(c, sp_s0, aux0, i0, p) ==> sp_sM.ok && exists auxM :: GenericStateInvariant(c, sp_sM, auxM, iM, p)
+}
+
+function method sp_code_GenericUnrolledChunk(start:int, end:int, p:GenericCodeParameters) : codes
+    requires 0 <= start <= end <= GenericIterationCount();
+    decreases end - start;
+{
+    if start == end then
+        CNil()
+    else
+        sp_CCons(GenericCodeIteration(start, p), sp_code_GenericUnrolledChunk(start+1, end, p))
+}
+
+function method sp_code_GenericUnrolled(p:GenericCodeParameters) : code
+{
+    Block(sp_code_GenericUnrolledChunk(0, GenericIterationCount(), p))
+}
+
+lemma sp_lemma_GenericUnrolledChunk(
+    sp_b0:sp_codes,
+    sp_s0:sp_state,
+    sp_sN:sp_state,
+    start:int,
+    end:int,
+    p:GenericCodeParameters
+    ) returns (
+    sp_bM:sp_codes,
+    sp_sM:sp_state
+    )
+    requires 0 <= start <= end <= GenericIterationCount();
+    requires sp_require(sp_b0, Block(sp_code_GenericUnrolledChunk(start, end, p)), sp_s0, sp_sN);
+    ensures  sp_ensure(sp_b0, sp_bM, sp_s0, sp_sM, sp_sN);
+    ensures  forall sp_id:sp_int, c:GenericConstantState, aux0:GenericAuxiliaryState {:trigger sp_trigger_GenericUnrolledChunk(sp_id, c, aux0)} ::
+                 sp_trigger_GenericUnrolledChunk(sp_id, c, aux0) ==> sp_spec_GenericUnrolledChunk(c, aux0, sp_s0, sp_sM, start, end, p);
+    ensures  GenericFramingInvariant(sp_s0, sp_sM);
+    decreases end - start;
+{
+    var sp_cM, sp_sM_preliminary;
+    sp_sM_preliminary, sp_cM, sp_bM := sp_lemma_block(sp_b0, sp_s0, sp_sN);
+    var sp_b1:sp_codes := sp_get_block(sp_cM);
+    assert sp_eval(Block(sp_bM), sp_sM_preliminary, sp_sN);
+
+    if start == end {
+        sp_sM := sp_lemma_empty(sp_s0, sp_sM_preliminary);
+        reveal_sp_spec_GenericUnrolledChunk();
+        forall sp_id:sp_int, c:GenericConstantState, aux0:GenericAuxiliaryState {:trigger sp_trigger_GenericUnrolledChunk(sp_id, c, aux0)}
+            | sp_trigger_GenericUnrolledChunk(sp_id, c, aux0)
+            ensures sp_spec_GenericUnrolledChunk(c, aux0, sp_s0, sp_sM, start, end, p);
+        {
+            var auxM := aux0;
+            if sp_s0.ok && GenericStateInvariant(c, sp_s0, aux0, start, p)
+            {
+                assert GenericStateInvariant(c, sp_sM, auxM, end, p);
+            }
+        }
+        assert GenericFramingInvariant(sp_s0, sp_sM);
+        return;
+    }
+
+    var sp_bL, sp_sL := sp_lemma_GenericIterationPreservesInvariants(sp_b1, sp_s0, sp_sM_preliminary, start, p);
+
+    var sp_bL_expanded := Block(sp_CCons(Block(sp_bL), CNil()));
+    assert sp_eval(sp_bL_expanded, sp_sL, sp_sM_preliminary) by
+    {
+        if sp_sL.ok {
+            var sL := to_state(sp_sL);
+            var sM := to_state(sp_sM_preliminary);
+            reveal_evalCodeOpaque();
+            assert evalCode(sp_bL_expanded.block.hd, sL, sM);
+            assert evalBlock(sp_bL_expanded.block.tl, sM, sM);
+            assert evalBlock(sp_bL_expanded.block, sL, sM);
+        }
+    }
+
+    ghost var sp_bM';
+    sp_bM', sp_sM := sp_lemma_GenericUnrolledChunk(sp_bL_expanded.block, sp_sL, sp_sM_preliminary, start+1, end, p);
+    sp_sM := sp_lemma_empty(sp_sM, sp_sM_preliminary);
+    assert sp_eval(Block(sp_bM), sp_sM, sp_sN);
+    assert sp_ensure(sp_b0, sp_bM, sp_s0, sp_sM, sp_sN);
+    lemma_GenericFramingInvariantTransitivity(sp_s0, sp_sL, sp_sM);
+
+    reveal_sp_spec_GenericUnrolledChunk();
+    forall sp_id:sp_int, c:GenericConstantState, aux0:GenericAuxiliaryState {:trigger sp_trigger_GenericUnrolledChunk(sp_id, c, aux0)}
+        | sp_trigger_GenericUnrolledChunk(sp_id, c, aux0)
+        ensures sp_spec_GenericUnrolledChunk(c, aux0, sp_s0, sp_sM, start, end, p);
+    {
+        assert sp_trigger_GenericUnrolledChunk(sp_id, c, aux0);
+        if sp_s0.ok && GenericStateInvariant(c, sp_s0, aux0, start, p)
+        {
+            assert sp_sL.ok;
+            var auxL :| GenericStateInvariant(c, sp_sL, auxL, start+1, p);
+            assert sp_trigger_GenericUnrolledChunk(sp_id, c, auxL);
+            assert sp_spec_GenericUnrolledChunk(c, auxL, sp_sL, sp_sM, start+1, end, p);
+            assert sp_spec_GenericUnrolledChunk(c, aux0, sp_s0, sp_sM, start, end, p);
+        }
+    }
+}
+
+lemma sp_lemma_GenericUnrolled(
+    sp_b0:sp_codes,
+    sp_s0:sp_state,
+    sp_sN:sp_state,
+    p:GenericCodeParameters
+    ) returns (
+    sp_bM:sp_codes,
+    sp_sM:sp_state
+    )
+    requires sp_require(sp_b0, sp_code_GenericUnrolled(p), sp_s0, sp_sN);
+    ensures  sp_ensure(sp_b0, sp_bM, sp_s0, sp_sM, sp_sN);
+    ensures  forall sp_id:sp_int, c:GenericConstantState, aux0:GenericAuxiliaryState {:trigger sp_trigger_GenericUnrolledChunk(sp_id, c, aux0)} ::
+                 sp_trigger_GenericUnrolledChunk(sp_id, c, aux0) ==> sp_spec_GenericUnrolledChunk(c, aux0, sp_s0, sp_sM, 0, GenericIterationCount(), p);
+    ensures  GenericFramingInvariant(sp_s0, sp_sM);
+{
+    sp_bM, sp_sM := sp_lemma_GenericUnrolledChunk(sp_b0, sp_s0, sp_sN, 0, GenericIterationCount(), p);
+}
+    
+}
