verified/Maybe.dfy
@@ -1,7 +1,9 @@
+module Maybe {
 datatype Maybe<T> = Nothing | Just(v: T)
 
 function method fromJust<T>(x: Maybe<T>): T
     requires x.Just?
 {
     x.v
+}
 }
