verified/sha/Seqs.s.dfy
@@ -1,6 +1,6 @@
 // REQUIRES-ANY: TEST, COLLECTIONS
 // RUN: %DAFNY /compile:0 %s %DARGS
-
+module Seqs_s {
 function last<T>(s:seq<T>):T
     requires |s| > 0;
 {
@@ -12,4 +12,5 @@ function all_but_last<T>(s:seq<T>):seq<T>
     ensures  |all_but_last(s)| == |s| - 1;
 {
     s[..|s|-1]
+}
 }
