verified/sha/sha256-refined-helpers.i.dfy
@@ -5,6 +5,16 @@ include "../sha/sha256.i.dfy"
 include "../sha/bit-vector-lemmas.i.dfy"
 include "../ARMdecls.gen.dfy"
 
+module sha256_refined_helpers_i {
+
+import opened sha256_refined_helpers_i_ARMspartan = ARMspartan 
+import opened sha256_refined_helpers_i_words_and_bytes_s = words_and_bytes_s 
+import opened sha256_refined_helpers_i_kom_common_s = kom_common_s 
+import opened sha256_refined_helpers_i_sha256_i = sha256_i
+import opened sha256_refined_helpers_i_bit_vector_lemmas_i = bit_vector_lemmas_i
+import opened sha256_refined_helpers_i_ARMdecls = ARMdecls 
+
+
 lemma lemma_BitwiseAdd32Associates3'(x1:word, x2:word, x3:word)
     ensures BitwiseAdd32(BitwiseAdd32(x1, x2), x3) == BitwiseAdd32(x1, BitwiseAdd32(x2, x3));
 {
@@ -55,4 +65,6 @@ lemma lemma_BitwiseAdd32Associates4(x1:word, x2:word, x3:word, x4:word, result:w
             { lemma_BitwiseAdd32Associates3(x1, x3, x2); }
         BitwiseAdd32(BitwiseAdd32(BitwiseAdd32(x1, x2), x3), x4);
     }
+}
+
 }
